HMAC: update the specification to use the real CT-SHA2

crypto_hst/hmac/HMAC.B.fst
@@ -13,33 +13,45 @@ open Hacl.SBuffer
 open Hacl.Operations
 open Hacl.Conversions
 
+module U8 = FStar.UInt8
+module S8 = Hacl.UInt8
+module U32 = FStar.UInt32
+module S32 = Hacl.UInt32
+module U64 = FStar.UInt64
+module S64 = Hacl.UInt64
+module SB = Hacl.SBuffer
 
 
 (* Define base types *)
+let s8 = Hacl.UInt8.t
 let u32 = FStar.UInt32.t
+let s32 = Hacl.UInt32.t
 let u64 = FStar.UInt64.t
 let s64 = Hacl.UInt64.t
-let s32 = Hacl.UInt32.t
-let s8 = Hacl.UInt8.t
 let uint32s = Hacl.SBuffer.u32s
 let bytes = Hacl.SBuffer.u8s
 
 
 (* Define operators *)
-let op_At_Plus = UInt32.add
+let op_At_Plus = U32.add_mod
 
 
 (* Define parameters *)
 let hash = Hash.Sha256.sha256
-let hl = 32ul
-let bl = 64ul
+let hashsize = Hash.Sha256.hashsize
+let blocksize = Hash.Sha256.blocksize
+let hl = hashsize
+let bl = blocksize
+
 
 
 (* Define a function to wrap the key length after bl bits *)
-val wrap_key : (okey:bytes{ length okey = v bl}) -> (key:bytes {disjoint okey key}) -> (keylen :u32 { length key = v keylen })
-               -> STL unit
-                     (requires (fun h -> live h okey /\ live h key))
-                     (ensures  (fun h0 _ h1 -> live h1 okey /\ live h1 key /\ modifies_1 okey h0 h1))
+val wrap_key : (okey   :bytes{length okey = U32.v bl}) ->
+               (key    :bytes{length key % (U32.v bl) = 0 /\ disjoint okey key}) ->
+               (keylen :u32  {U32.v keylen <= length key})
+  -> STL unit
+        (requires (fun h -> live h okey /\ live h key))
+        (ensures  (fun h0 _ h1 -> live h1 okey /\ live h1 key /\ modifies_1 okey h0 h1))
 
 let wrap_key okey key keylen =
   if gt keylen bl then
@@ -48,18 +60,32 @@ let wrap_key okey key keylen =
     blit key 0ul okey 0ul keylen
 
 
+
+(* Size and positions of objects in memb *)
+let size_ipad = bl
+let size_opad = bl
+let size_okey = bl
+let size_s3 = bl @+ bl
+let size_s6 = bl @+ bl
+let size_memb = size_ipad @+ size_opad @+ size_okey @+ size_s3 @+ size_s6
+
+let pos_ipad = 0ul
+let pos_opad = bl
+let pos_okey = bl @+ bl
+let pos_s3 = bl @+ bl @+ bl
+let pos_s6 = bl @+ bl @+ bl @+ bl @+ bl
+
+
 (* Define the internal function *)
-val hmac_core' :(memb    :bytes) ->
-                  (mac     :bytes { length mac = v hl /\ disjoint mac memb }) ->
-                  (key     :bytes { disjoint key memb }) ->
-                  (keylen  :u32   { length key = v keylen }) ->
-                  (data    :bytes { disjoint data memb /\ disjoint mac data }) ->
-                  (datalen :u32   { length data = v datalen /\ v datalen + v bl <= pow2 32
-                                  /\ length memb = v bl + v bl + v bl + (v bl + v datalen) + (v bl + v hl)})
+val hmac_core' :  (memb    :bytes {length memb = U32.v size_memb}) ->
+                  (mac     :bytes {length mac = U32.v hl /\ disjoint mac memb }) ->
+                  (key     :bytes {length key % (U32.v bl) = 0 /\ disjoint key memb }) ->
+                  (keylen  :u32   {U32.v keylen <= length key}) ->
+                  (data    :bytes {length data % (U32.v bl) = 0 /\ disjoint data memb /\ disjoint mac data }) ->
+                  (datalen :u32   {U32.v datalen <= length data /\ U32.v datalen + U32.v bl <= pow2 32})
                   -> STL unit
                         (requires (fun h -> live h memb /\ live h mac /\ live h data /\ live h key))
                         (ensures  (fun h0 r h1 -> live h1 memb /\ live h1 mac /\ modifies_2 memb mac h0 h1))
-
 
 let hmac_core' memb mac key keylen data datalen =
 
@@ -67,17 +93,17 @@ let hmac_core' memb mac key keylen data datalen =
   (**) let h0 = HST.get() in
 
   (* Set initial values for ipad and opad *)
-  let ipad = sub memb 0ul bl in
-  setall ipad bl 0x36uy;
-  let opad = sub memb bl bl in
-  setall opad bl 0x5cuy;
+  let ipad = sub memb pos_ipad size_ipad in
+  setall ipad size_ipad (uint8_to_sint8 0x36uy);
+  let opad = sub memb pos_opad size_opad in
+  setall opad size_opad (uint8_to_sint8 0x5cuy);
 
   (* Create the wrapped key location *)
-  let okey = sub memb (bl @+ bl) bl in
+  let okey = sub memb pos_okey size_okey in
 
   (* Create the working emplacements *)
-  let s3 = sub memb (bl @+ bl @+ bl) (bl @+ datalen) in
-  let s6 = sub memb (bl @+ bl @+ bl @+ bl @+ datalen) (bl @+ hl) in
+  let s3 = sub memb pos_s3 size_s3 in
+  let s6 = sub memb pos_s6 size_s6 in
 
   (* Step 1: make sure the key has the proper length *)
   wrap_key okey key keylen;
@@ -88,7 +114,7 @@ let hmac_core' memb mac key keylen data datalen =
 
   (* Step 3: append data to "result of step 2" *)
   blit s2 0ul s3 0ul bl;
-  blit data 0ul s3 bl datalen;
+  blit data 0ul s3 bl bl;
 
   (* Step 4: apply H to "result of step 3" *)
   let s4 = s2 in
@@ -100,7 +126,7 @@ let hmac_core' memb mac key keylen data datalen =
 
   (* Step 6: append "result of step 4" to "result of step 5" *)
   blit s5 0ul s6 0ul bl;
-  blit s4 0ul s6 bl hl;
+  blit s4 0ul s6 bl bl;
 
   (**) let h1 = HST.get() in
   (**) assert(modifies_1 memb h0 h1);
@@ -118,21 +144,21 @@ let hmac_core' memb mac key keylen data datalen =
 
 
 (* Define the main function *)
-val hmac_core : (mac     :bytes { length mac = v hl }) ->
-                  (key     :bytes { disjoint key mac }) ->
-                  (keylen  :u32   { length key = v keylen }) ->
-                  (data    :bytes { disjoint mac data }) ->
-                  (datalen :u32   {5 * v bl + v hl + v datalen < pow2 32 /\ length data = v datalen /\ v datalen + v bl <= pow2 32})
-                  -> STL unit
-                        (requires (fun h -> live h mac /\ live h data /\ live h key))
-                        (ensures  (fun h0 r h1 -> live h1 mac /\ modifies_1 mac h0 h1))
+val hmac_core : (mac     :bytes {length mac = U32.v hl}) ->
+                (key     :bytes {length key % (U32.v bl) = 0}) ->
+                (keylen  :u32   {U32.v keylen <= length key}) ->
+                (data    :bytes {length data % (U32.v bl) = 0 /\ disjoint mac data}) ->
+                (datalen :u32   {U32.v datalen <= length data /\ U32.v datalen + U32.v bl <= pow2 32})
+  -> STL unit
+        (requires (fun h -> live h mac /\ live h data /\ live h key))
+        (ensures  (fun h0 r h1 -> live h1 mac /\ modifies_1 mac h0 h1))
 
 let hmac_core mac key keylen data datalen =
 
   (** Push a new frame *)
   (**) push_frame();
 
-  let memblen = bl @+ bl @+ bl @+ (bl @+ datalen) @+ (bl @+ hl) in
+  let memblen = size_memb in
   let memb = create (uint8_to_sint8 0uy) memblen in
 
   hmac_core' memb mac key keylen data datalen;
@@ -142,13 +168,13 @@ let hmac_core mac key keylen data datalen =
 
 
 (* Exposing SHA2-256 for test vectors *)
-val hmac_sha256 : (mac     :bytes { length mac = v hl }) ->
-                  (key     :bytes { disjoint key mac }) ->
-                  (keylen  :u32   { length key = v keylen }) ->
-                  (data    :bytes { disjoint mac data }) ->
-                  (datalen :u32   {5 * v bl + v hl + v datalen < pow2 32 /\ length data = v datalen /\ v datalen + v bl <= pow2 32})
-                  -> STL unit
-                        (requires (fun h -> live h mac /\ live h data /\ live h key))
-                        (ensures  (fun h0 r h1 -> live h1 mac /\ modifies_1 mac h0 h1))
+val hmac_sha256 : (mac     :bytes {length mac = U32.v hl}) ->
+                  (key     :bytes {length key % (U32.v bl) = 0}) ->
+                  (keylen  :u32   {U32.v keylen <= length key}) ->
+                  (data    :bytes {length data % (U32.v bl) = 0 /\ disjoint mac data}) ->
+                  (datalen :u32   {U32.v datalen <= length data /\ U32.v datalen + U32.v bl <= pow2 32})
+  -> STL unit
+        (requires (fun h -> live h mac /\ live h data /\ live h key))
+        (ensures  (fun h0 r h1 -> live h1 mac /\ modifies_1 mac h0 h1))
 
 let hmac_sha256 mac key keylen data datalen = hmac_core mac key keylen data datalen
